- Ejercicios 1: Simplifica
```math
\begin{align}
(-3)^3x^0y^3 &= -27y^3 \tag{1.1} \\
4^2xy^2 &= 16xy^2 \tag{1.2} \\
-4^2x^2y^0z^3 &= -16x^2z^3 \tag{1.3} \\
\frac{3x^3z^2}{2y^0} &= \frac{3x^3z^2}{2} \tag{1.4}
\end{align}
```
- Ejercicios 2: Simplifica
```math
\begin{align}
2^{-1} &= \frac{1}{2} \tag{2.1} \\
3^{-3} &= \frac{1}{27} \tag{2.2} \\
x^{-2} &= \frac{1}{x^2} \tag{2.3} \\
\left(\frac{2}{3}\right)^{-2} &= \frac{9}{4} \tag{2.4} \\
\frac{5}{y^{-5}} &= 5y^5 \tag{2.5} \\
\frac{x^{-2}}{y^{-5}} &= \frac{y^5}{x^2} \tag{2.6}
\end{align}
```
- Ejercicios 3: Simplifica
```math
\begin{align}
-5^2x^2y^{-3} &= \frac{-25x^2}{y^{3}} \tag{3.1} \\
(-4)^2x^{-2}y^0x^{-3} &= \frac{16}{x^{5}} \tag{3.2} \\
4^{-2}x^{-1}y^2 &= \frac{y^2}{16x} \tag{3.3} \\
\frac{8x^{-3}x^2}{y^{-4}} &= \frac{8y^4}{x} \tag{3.4}
\end{align}
```
- Simplifica aplicando leyes de exponentes:
```math
\begin{align}
9^{15}9^3 &= 9^{15+3} = 9^{18} \tag{4.1} \\
x^3x^{12}x &= x^{3+12+1} = x^{16} \tag{4.2} \\
x^2 + x^5 &= x^2(1 + x^3) \tag{4.3} \\
x^{-2}x^{-3}x^{-1}x^5 &= x^{-2-3-1+5} = x^{-1} \tag{4.4} 
\end{align}
```
- Simplifica aplicando leyes de exponentes:
```math
\begin{align}
(m^4)^5 &= m^{4 \cdot 5} = m^{20} \tag{5.1} \\
(3^{12})^3 &= 3^{12 \cdot 3} = 3^{36} \tag{5.2} \\
(x^9)^0 &= 1 \tag{5.3} \\
(4^3)^{-1} &= 4^{-3 \cdot 1} = 4^{-3} = \frac{1}{4^3} = \frac{1}{64} \tag{5.4}
\end{align}
```
- Simplifica aplicando leyes de exponentes:
```math
\begin{align}
(xy)^3 &= x^3y^3 \tag{6.1} \\
(2x)^5 &= 32x^5 \tag{6.2} \\
(3x^4y^5)^{-3} &= \frac{1}{27x^{12}y^{15}} \tag{6.3} \\
(x+y)^2 &= x^2 + 2xy + y^2 \tag{6.4}
\end{align}
```
- Simplifica aplicando leyes de exponentes:
```math
\begin{align}
\frac{x^4}{x^2} &= x^{4-2} = x^2 \tag{7.1} \\
\frac{y^{19}}{y^{18}} &= y^{19-18} = y \tag{7.2} \\
\frac{m^{13}}{m^{23}} &= m^{13-23} = m^{-10} = \frac{1}{m^{10}} \tag{7.3} \\
\frac{x^{63}}{x^{63}} &= x^{63-63} = 1 \tag{7.4}
\end{align}
```
- Simplifica aplicando leyes de exponentes:
```math
\begin{align}
\left(\frac{m}{n}\right)^5 &= \frac{m^5}{n^5} \tag{8.1} \\
\left(\frac{x}{y^4}\right)^{-8} &= \frac{y^{32}}{x^8} \tag{8.2} \\
\left(\frac{x^6}{2}\right)^3 &= \frac{x^{18}}{8} \tag{8.3} \\
\left(\frac{x^7}{y^5}\right)^{-3} &= \frac{y^{15}}{x^{21}} \tag{8.4}
\end{align}
```
