Simplifica aplicando leyes de exponentes:
1. $$(m^4)^5 = m^{4 \cdot 5} = m^{20}$$
2. $$(3^{12})^3 = 3^{12 \cdot 3} = 3^{36}$$
3. $$(x^9)^0 = x^{9 \cdot 0} = x^0 = 1$$
4. $$(4^3)^{-1} = 4^{3 \cdot -1} = 4^{-3} = \frac{1}{4^3} = \frac{1}{64}$$

Simplifica aplicando leyes de exponentes:
1. $$(x y)^3 = x^3 y^3$$
2. $$(2 x)^5 = 32 x^5$$
3. $$(3 x 4 y 5)^{-3} = \frac{1}{3^3 \cdot 4^3 \cdot 5^3 x^3 y^3}$$
4. $$(x + y)^2 = x^2 + 2xy + y^2$$

Simplifica aplicando leyes de exponentes:

1. $$\frac{x^4}{x^2} = x^{4-2} = x^2$$
2. $$\frac{y^{19}}{y^{18}} = y^{19-18} = y$$
3. $$\frac{x^{63}}{x^{63}} = x^{63-63} = x^0 = 1$$

Simplifica aplicando leyes de exponentes:

1. $$(\frac{m}{n})^5 = \frac{m^5}{n^5}$$
2. $$(\frac{x}{y^4})^{-8} = \frac{y^{32}}{x^8}$$
3. $$(\frac{x^6}{2})^3 = \frac{x^{18}}{8}$$
4. $$(\frac{x^7}{y^5})^{-3} = \frac{y^{15}}{x^{21}}$$

